work in progress, need to clean up Program.i...

Splinter/Allocation.i.dfy
@@ -3,27 +3,7 @@
 
 // XXX --- QUESTION: Is this a module that just allocates disk blocks?
 module AllocationMod {
-  type AU = nat
-  datatype CU = CU(au: AU, offset: nat)
-  type UninterpretedDiskPage
-
-  function DiskSizeInAU() : (s:nat)
-    ensures 1<=s
-
-  function AUSizeInCUs() : (s:nat)
-    ensures 2<=s  // TODO(jonh): explain why
-
-  function {:opaque} CUsInDisk() : set<CU>
-  {
-    set au,offset | 0<=au<DiskSizeInAU() && 0<=offset<AUSizeInCUs() :: CU(au,offset)
-  }
-
-  predicate ValidCU(cu: CU) {
-    && 0 <= cu.au < DiskSizeInAU()
-    && 0 <= cu.offset < AUSizeInCUs()
-  }
-
-  type DiskView = map<CU, UninterpretedDiskPage>
+  import opened DiskTypesMod
 
   // TODO(jonh): robj points out we should have a ValidView first, then fullness later.
   predicate FullView(dv: DiskView) {
