Splinter/BetreeInterp.i.dfy
@@ -15,6 +15,7 @@ module BetreeInterpMod {
   import opened Options
   import opened MessageMod
   import opened InterpMod
+  import opened DiskTypesMod
   import opened AllocationMod
   import opened MsgSeqMod
   import IndirectionTableMod
@@ -33,7 +34,7 @@ module BetreeInterpMod {
   predicate ValidLookup(v: Variables, cache: CacheIfc.Variables, key: Key, lookup: Lookup)
     // TODO
 
-  function IMKey(v: Variables, cache: CacheIfc.Variables, sb: Superblock, key: Key) : Message
+  function IMKey(v: Variables, cache: CacheIfc.Variables, key: Key) : Message
   {
     if exists lookup :: ValidLookup(v, cache, key, lookup)
     then
@@ -43,10 +44,22 @@ module BetreeInterpMod {
       MessagePut(key, DefaultValue())
   }
 
-  function IM(v: Variables, cache: CacheIfc.Variables, sb: Superblock) : (i:Interp)
+  function IM(cache: CacheIfc.Variables, v: Variables) : (i:Interp)
     ensures i.WF()
   {
-    Interp(imap key | key in AllKeys() :: IMKey(v, cache, sb, key), sb.endSeq)
+    Interp(imap key | key in AllKeys() :: IMKey(v, cache, key), v.nextSeq) // check v.nextSeq used to be sb.endSeq
+  }
+
+  function IMStable(cache: CacheIfc.Variables, sb: Superblock) : (i:Interp)
+    ensures i.WF()
+  {
+    if exists indTbl :: IndirectionTableMod.DurableAt(indTbl, cache, sb.indTbl)
+    then
+      var indTbl :| IndirectionTableMod.DurableAt(indTbl, cache, sb.indTbl);
+      var v := Variables(indTbl, map[], sb.endSeq, Frozen.Idle);
+      IM(cache, v)
+    else
+      InterpMod.Empty()
   }
 
   // Imagine what the disk would look like if we were running and haven't
@@ -59,7 +72,7 @@ module BetreeInterpMod {
     then InterpMod.Empty()
     else
       var pretendVariables := Variables(indTbl.value, map[], sb.endSeq, Idle);
-      IM(pretendVariables, cache, sb)
+      IM(cache, pretendVariables)
   }
 
   function IReadsKey(v: Variables, cache: CacheIfc.Variables, sb: Superblock, key: Key) : set<CU> {
@@ -87,12 +100,12 @@ module BetreeInterpMod {
 
   lemma Framing(v: Variables, cache0: CacheIfc.Variables, cache1: CacheIfc.Variables, sb:Superblock)
     requires DiskViewsEquivalentForSet(cache0.dv, cache1.dv, IReads(v, cache0, sb))
-    ensures IM(v, cache0, sb) == IM(v, cache1, sb)
+    ensures IM(cache0, v) == IM(cache1, v)
   {
     // TODO I'm surprised this proof passes easily.
     // narrator: It doesn't.
     forall key | key in AllKeys()
-      ensures IMKey(v, cache0, sb, key) == IMKey(v, cache1, sb, key)
+      ensures IMKey(v, cache0, key) == IMKey(v, cache1, key)
     {
       var le0 := exists lookup0 :: ValidLookup(v, cache0, key, lookup0);
       var le1 := exists lookup1 :: ValidLookup(v, cache1, key, lookup1);
@@ -110,26 +123,26 @@ module BetreeInterpMod {
         var lookup0 :| ValidLookup(v, cache0, key, lookup0);
         var lookup1 :| ValidLookup(v, cache1, key, lookup1);
         calc {
-          IMKey(v, cache0, sb, key);
+          IMKey(v, cache0, key);
             { assume false; } // var|
           LookupToMessage(lookup0);
             { assume false; } // framing
           LookupToMessage(lookup1);
             { assume false; } // var|
-          IMKey(v, cache1, sb, key);
+          IMKey(v, cache1, key);
         }
       } else {
         calc {
-          IMKey(v, cache0, sb, key);
+          IMKey(v, cache0, key);
           MessagePut(key, DefaultValue());
-          IMKey(v, cache1, sb, key);
+          IMKey(v, cache1, key);
         }
       }
     }
   }
 
   lemma PutEffect(v: Variables, v': Variables, cache: CacheIfc.Variables, cache': CacheIfc.Variables, sb: Superblock, key: Key, value: Value, sk: Skolem)
-    ensures IM(v', cache', sb) == IM(v, cache, sb).Put(key, MessagePut(key, value))
+    ensures IM(cache', v') == IM(cache, v).Put(key, MessagePut(key, value))
   {
     assume false; // This is hard to prove -- we need to finish a tree
   }
