Splinter/IOSystem.s.dfy
@@ -6,27 +6,62 @@ include "../lib/Base/MapRemove.s.dfy"
 include "../lib/Checksums/CRC32C.s.dfy"
 include "AsyncDisk.s.dfy"
 include "AsyncDiskProgram.s.dfy"
+include "DiskTypes.s.dfy"
+
 
 // The Specification for the entire IOSystem (Disk + Program)
 abstract module IOSystem {
-  import AllocationMod
+  import DiskTypesMod
   import D = AsyncDisk
   import P : AsyncDiskProgram
   import opened NativeTypes
+  import AsyncMapSpecMod
 
   type DiskOp = P.DiskOp
-  datatype Variables = Variables(program: P.Variables, disk: D.Variables)
+  datatype Variables = Variables(program: P.Variables, disk: D.Variables, requests: set<AsyncMapSpecMod.Request>, replies: set<AsyncMapSpecMod.Reply>)
   type UIOp = P.UIOp
 
   datatype Step =
     | MachineStep(dop: DiskOp)
     | DiskInternalStep(step: D.InternalStep)
     | CrashStep
+    | AcceptRequestStep
+    | DeliverReplyStep
+
+
+  predicate AcceptRequest(s: Variables, s': Variables, uiop: UIOp)
+  {
+    && uiop.OperateOp?
+    && uiop.baseOp.RequestOp?
+    && s' == s.(requests := s.requests + {uiop.baseOp.req})
+  }
+
+  predicate DeliverReply(s: Variables, s': Variables, uiop: UIOp)
+  {
+
+    && uiop.OperateOp?
+    && uiop.baseOp.ReplyOp?
+    && uiop.baseOp.reply in s.replies
+    && s' == s.(replies := s.replies - {uiop.baseOp.reply})
+  }
 
   predicate Machine(s: Variables, s': Variables, uiop: UIOp, dop: DiskOp)
   {
+    && !uiop.CrashOp?
+    && (
+      if uiop.OperateOp? then
+        && uiop.baseOp.ExecuteOp?
+        && uiop.baseOp.req in s.requests
+        && uiop.baseOp.req.id == uiop.baseOp.reply.id
+        && s'.requests == s.requests - {uiop.baseOp.req}
+        && s'.replies == s.replies + {uiop.baseOp.reply}
+      else
+        && s'.requests == s.requests
+        && s'.replies == s.replies
+      )
     && P.Next(s.program, s'.program, uiop, dop)
     && D.Next(s.disk, s'.disk, dop)
+
   }
 
   predicate DiskInternal(s: Variables, s': Variables, uiop: UIOp, step: D.InternalStep)
@@ -34,6 +69,8 @@ abstract module IOSystem {
     && uiop.NoopOp?
     && s.program == s'.program
     && D.NextInternalStep(s.disk, s'.disk, step)
+    && s'.requests == s.requests
+    && s'.replies == s.replies
   }
 
   predicate Crash(s: Variables, s': Variables, uiop: UIOp)
@@ -41,6 +78,8 @@ abstract module IOSystem {
     && uiop.CrashOp?
     && P.Init(s'.program)
     && D.Crash(s.disk, s'.disk)
+    && s'.requests == {}
+    && s'.replies == {}
   }
 
   predicate NextStep(s: Variables, s': Variables, uiop: UIOp, step: Step)
@@ -49,12 +88,14 @@ abstract module IOSystem {
       case MachineStep(dop) => Machine(s, s', uiop, dop)
       case DiskInternalStep(step) => DiskInternal(s, s', uiop, step)
       case CrashStep => Crash(s, s', uiop)
+      case AcceptRequestStep => AcceptRequest(s, s', uiop)
+      case DeliverReplyStep => DeliverReply(s, s', uiop)
     }
   }
 
   predicate Init(v: Variables) {
     && P.Init(v.program)
-    && var dv:AllocationMod.DiskView :| true; // TODO: AsyncDisk has wrong type!
+    && var dv:DiskTypesMod.DiskView :| true; // TODO: AsyncDisk has wrong type!
     //&& P.Mkfs(v.disk.dv)
     && P.Mkfs(dv) // this init is only true once
   }
