Splinter/DiskTypes.s.dfy
@@ -1,0 +1,24 @@
+
+module DiskTypesMod {
+  type AU = nat
+  datatype CU = CU(au: AU, offset: nat)
+  type UninterpretedDiskPage
+
+  function DiskSizeInAU() : (s:nat)
+    ensures 1<=s
+
+  function AUSizeInCUs() : (s:nat)
+    ensures 2<=s  // TODO(jonh): explain why
+
+  function {:opaque} CUsInDisk() : set<CU>
+  {
+    set au,offset | 0<=au<DiskSizeInAU() && 0<=offset<AUSizeInCUs() :: CU(au,offset)
+  }
+
+  predicate ValidCU(cu: CU) {
+    && 0 <= cu.au < DiskSizeInAU()
+    && 0 <= cu.offset < AUSizeInCUs()
+  }
+
+  type DiskView = map<CU, UninterpretedDiskPage>
+}
