Splinter/RefinementProof.i.dfy
@@ -1,17 +1,26 @@
 include "IOSystem.s.dfy"
 include "ProgramInterp.i.dfy"
 include "ProofObligations.s.dfy"
+include "JournalInterp.i.dfy"
 
 module VeribetrIOSystem refines IOSystem {
   import P = ProgramMachineMod
 }
 
 module Proof refines ProofObligations {
-  import AllocationMod
+  import opened DiskTypesMod
   import MapSpecMod
   import InterpMod
   import ProgramInterpMod
   import ConcreteSystem = VeribetrIOSystem
+  import JournalMachineMod
+  import BetreeMachineMod
+  import JournalInterpMod
+
+
+  import BetreeInterpMod
+
+  import CacheIfc
 
   function I(v: ConcreteSystem.Variables) : CrashTolerantMapSpecMod.Variables
   {
@@ -23,6 +32,7 @@ module Proof refines ProofObligations {
     true
   }
 
+  // Remember that this is the init of a p
   lemma InitRefines(v: ConcreteSystem.Variables)
 //    requires ConcreteSystem.Init(v)
     ensures CrashTolerantMapSpecMod.Init(I(v))
@@ -39,11 +49,129 @@ module Proof refines ProofObligations {
 //    ensures ConcreteSystem.Inv(v')
   {}
 
-  lemma NextRefines(v: ConcreteSystem.Variables, v': ConcreteSystem.Variables, uiop: ConcreteSystem.UIOp)
-//    requires ConcreteSystem.Inv(v)
-//    requires ConcreteSystem.Next(v, v')
-//    ensures CrashTolerantMapSpecMod.Next(ConcreteSystem.I(v), ConcreteSystem.I(v'))
+  lemma BetreeInternalRefined(v: ConcreteSystem.P.Variables, v': ConcreteSystem.P.Variables, uiop: ConcreteSystem.UIOp, cacheOps : CacheIfc.Ops, pstep: ConcreteSystem.P.Step, sk: BetreeMachineMod.Skolem)
+      requires ConcreteSystem.P.NextStep(v, v', cacheOps, pstep)
+      requires pstep == ConcreteSystem.P.BetreeInternalStep(sk)
+      // Is this a problem with using imports?
+      ensures BetreeInterpMod.IM(v.cache, v.betree) ==
+       BetreeInterpMod.IM(v'.cache, v'.betree)
   {
+
+  }
+
+  lemma JournalInternalRefined(v: ConcreteSystem.P.Variables, v': ConcreteSystem.P.Variables, uiop: ConcreteSystem.UIOp, cacheOps : CacheIfc.Ops, pstep: ConcreteSystem.P.Step, sk: JournalMachineMod.Skolem)
+    requires ConcreteSystem.P.NextStep(v, v', cacheOps, pstep)
+    requires pstep == ConcreteSystem.P.JournalInternalStep(sk)
+    //requires BetreeInterpMod.IM(v.betree, v.cache, v.stableSuperblock.betree) == BetreeInterpMod.IM(v'.betree, v'.cache, v'.stableSuperblock.betree)
+    // eek .... this is ugly. But maybe the intuition is correct here?
+    ensures JournalInterpMod.IM(v.journal, v.cache, v.stableSuperblock.journal, BetreeInterpMod.IM(v.cache, v.betree)) ==
+      JournalInterpMod.IM(v'.journal, v'.cache, v'.stableSuperblock.journal, BetreeInterpMod.IM(v'.cache, v'.betree))
+  {
+
+    BetreeInterpMod.Framing(v.betree, v.cache, v'.cache, v.stableSuperblock.betree);
+
+    assert BetreeInterpMod.IM(v.cache, v.betree) == BetreeInterpMod.IM( v'.cache, v'.betree);
+
+  }
+
+// This is a ghost method
+  lemma MachineStepRefines(v: ConcreteSystem.Variables, v': ConcreteSystem.Variables, uiop: ConcreteSystem.UIOp, step : ConcreteSystem.Step)
+    requires Inv(v)
+    requires ConcreteSystem.Next(v, v', uiop)
+    requires ConcreteSystem.NextStep(v, v', uiop, step)
+    requires step.MachineStep?
+    ensures CrashTolerantMapSpecMod.Next(I(v), I(v'), uiop)
+  {
+     var cacheOps, pstep :| ConcreteSystem.P.NextStep(v.program, v'.program, cacheOps, pstep);
+    match pstep {
+      case RecoverStep(puts, newbetree) => {
+
+        assume CrashTolerantMapSpecMod.Next(I(v), I(v'), uiop);
+      }
+      case QueryStep(key, val, sk) => {
+
+        assume CrashTolerantMapSpecMod.Next(I(v), I(v'), uiop);
+      }
+      case PutStep(key, val, sk) => {
+
+        assume CrashTolerantMapSpecMod.Next(I(v), I(v'), uiop);
+      }
+      case JournalInternalStep(sk) => {
+
+        JournalInternalRefined(v.program, v'.program, uiop, cacheOps, pstep, sk);
+        var sb := ProgramInterpMod.ISuperblock(v.program.cache.dv);
+        if sb.Some?
+        {
+          assert ProgramInterpMod.IM(v.program) == ProgramInterpMod.IM(v'.program);
+          assert I(v) == I(v');
+          // Here the map is no op
+          assert CrashTolerantMapSpecMod.NextStep(I(v), I(v'), CrashTolerantMapSpecMod.NoopOp);
+          assert CrashTolerantMapSpecMod.Next(I(v), I(v'), uiop); // believes this i think
+        } else
+        {
+          var sb' := ProgramInterpMod.ISuperblock(v'.program.cache.dv);
+          assert sb'.None?;
+          // Doesn't believe this...
+          calc {
+            I(v);
+            I(v');
+          }
+          assert CrashTolerantMapSpecMod.NextStep(I(v), I(v'), CrashTolerantMapSpecMod.NoopOp); // this is a witness
+          assert CrashTolerantMapSpecMod.Next(I(v), I(v'), CrashTolerantMapSpecMod.NoopOp);
+          assert CrashTolerantMapSpecMod.Next(I(v), I(v'), uiop);
+          assert uiop == CrashTolerantMapSpecMod.NoopOp;
+        }
+
+      }
+      case BetreeInternalStep(sk) => {
+          BetreeInternalRefined(v.program, v'.program, uiop, cacheOps, pstep, sk);
+
+          //
+
+          assume CrashTolerantMapSpecMod.NextStep(I(v), I(v'), CrashTolerantMapSpecMod.NoopOp);
+          assert CrashTolerantMapSpecMod.Next(I(v), I(v'), uiop);  // believes this i think
+      }
+      case ReqSyncStep(syncReqId) => {
+
+          assume CrashTolerantMapSpecMod.Next(I(v), I(v'), uiop);
+      }
+      case CompleteSyncStep(syncReqId) => {
+        assume CrashTolerantMapSpecMod.Next(I(v), I(v'), uiop);
+      }
+      case CommitStartStep(seqBoundary) => {
+
+          assume CrashTolerantMapSpecMod.Next(I(v), I(v'), uiop);
+      }
+      case CommitCompleteStep() => {
+
+          assume CrashTolerantMapSpecMod.Next(I(v), I(v'), uiop);
+      }
+    }
+
+  }
+
+  lemma NextRefines(v: ConcreteSystem.Variables, v': ConcreteSystem.Variables, uiop: ConcreteSystem.UIOp)
+  // requires Inv(v)
+  // requires ConcreteSystem.Next(v, v', uiop)
+  // ensures CrashTolerantMapSpecMod.Next(I(v), I(v'), uiop)
+  {
+    // cases to anyalze
+
+    // choose a step such that statifieds NextStep
+    var step :| ConcreteSystem.NextStep(v, v', uiop, step);
+
+    match step {
+      case MachineStep(_) => {
+          MachineStepRefines(v, v', uiop, step);
+          assert CrashTolerantMapSpecMod.Next(I(v), I(v'), uiop);
+        }
+      case DiskInternalStep(step) => {
+          assume  CrashTolerantMapSpecMod.Next(I(v), I(v'), uiop);
+      }
+      case CrashStep => {
+        assume  CrashTolerantMapSpecMod.Next(I(v), I(v'), uiop);
+      }
+    }
 
   }
 }
